Hs/Metatheory/Preservation.lean
@@ -1,29 +1,171 @@
-import Hs.Compile
+import Hs.CompileJ
 
 
 @[simp]
 abbrev CompileCtxWfType : (v : CompileVariant) -> (Γ : Ctx HsTerm) -> (CompileJArgs v Γ) -> Prop
-| .term => λ Γ => λ ⟨τ , k ; j, τ'⟩ => ∀ Γ',
-  (k = `★) ->  CompileJ .term Γ ⟨τ, k ; j, τ'⟩ -> CompileJ .ctx Γ Γ' ->  Γ' ⊢ τ' : ★
-  -- ∨ (k = `□ ->  Compile .term Γ (⟨τ, k ; j⟩, τ') ->  Compile .ctx Γ Γ' ->  Γ' ⊢ τ' : □)
+| .term => λ Γ => λ ⟨t , τ ; j , t'⟩ => ∀ Γ' τ',
+  CompileJ .ctx Γ Γ' ->
+  CompileJ .term Γ ⟨t, τ; j, t'⟩ ->
+  (jk : Γ ⊢s τ : `★) ->
+  CompileJ .type Γ ⟨τ, `★; jk, τ'⟩ ∧ (Γ' ⊢ t' : τ')
+| .type => λ Γ => λ ⟨τ , k ; j , τ'⟩ => ∀ Γ',
+  k = `★ ->
+  CompileJ .ctx Γ Γ' ->
+  CompileJ .type Γ ⟨τ, k; j, τ'⟩ ->
+  (jk : Γ ⊢s k : `□) ->
+  CompileJ .kind Γ ⟨k, `□; jk, ★⟩ ∧  (Γ' ⊢ τ' : ★)
+| .kind => λ Γ => λ ⟨k , ki ; j , k'⟩ => ∀ Γ',
+  ki = `□ ->
+  CompileJ .ctx Γ Γ' ->
+  CompileJ .kind Γ ⟨k, ki; j, k'⟩ ->
+  (Γ' ⊢ k' : □)
+
 | .ctx => λ Γ => λ Γ' => ⊢s Γ -> CompileJ .ctx Γ Γ' -> ⊢ Γ'
 
-theorem compile_wf_ctx :
- CompileJ v Γ idx -> CompileCtxWfType v Γ idx := by sorry
--- by
--- intro j; induction j <;> simp at *;
--- case _ =>intros; apply Judgment.wfnil;
--- all_goals (intro j c; cases j; cases c)
+theorem compile_preserves_validctors :
+  (j : Γ ⊢s τ : `★) ->
+  ValidHsCtorType Γ τ ->
+  CompileJ .ctx Γ Γ' ->
+  CompileJ .type Γ ⟨τ, `★; j, τ'⟩ ->
+  ValidCtorType Γ' τ' := by
+intros j1 j2 j3 j4;
+induction j2;
+case _ v =>
+  apply ValidCtorType.refl;
+  unfold HsValidHeadVariable at v;
+  unfold ValidHeadVariable; sorry
+case _ => sorry
+case _ => sorry
+case _ => sorry
+
+
+
+theorem compile_preserves_typing :
+ CompileJ v Γ idx -> CompileCtxWfType v Γ idx :=
+by
+intro j; induction j <;> simp at *;
+all_goals try (intro wf cc; cases cc; cases wf)
+case _ => apply Judgment.wfnil
+case _ ih cc wf =>
+  apply Judgment.wfempty (ih wf cc);
+case _  Γ' j c1 c2 ih1 ih2 _ _ j1 wf _ =>
+  apply Judgment.wftype;
+  have ih2' := ih2 Γ' c2 c1 (HsJudgment.ax wf);
+  cases ih2'; assumption
+  apply ih1 wf c2
+case _ Γ' j1 c1 c2 ih1 ih2 j2 c3 c4 wf j4 =>
+  apply Judgment.wfkind;
+  apply ih2 Γ' c2 c1
+  apply ih1 wf c2
+case _ Γ' j1 c1 c2 ih1 ih2 j2 c3 c4 wf j4 =>
+  apply Judgment.wfdatatype
+  apply ih2 Γ' c2 c1
+  apply ih1 wf c2
+case _ Γ' j1 c1 c2 ih1 ih2 j2 c3 c4 wf j3 j4 =>
+  apply Judgment.wfctor;
+  have ih2' := ih2 Γ' c2 c1 (HsJudgment.ax wf);
+  cases ih2'; assumption;
+  apply ih1 wf c2
+  apply compile_preserves_validctors j1 j4 c2 c1
+case _ A' _ Γ' j1 j2 c1 c2 c3 ih1 ih2 ih3 j3 j4 c4 c5 c6 wf j5 j6 =>
+  apply Judgment.wfterm;
+  have ih3' := ih3 Γ' c3 c1 (HsJudgment.ax wf); cases ih3'; assumption
+  have ih1' := ih1 Γ' A' c3 c2 j1;
+  cases ih1'; assumption;
+  apply ih2 wf c3
+
+all_goals try (intro Γ' cc c1)
+case _ wf =>
+  sorry
+case _ => sorry
+case _ => sorry
+case _ => sorry
+case _ => sorry
+case _ => sorry
+case _ => sorry
+case _ => sorry
+case _ => sorry
+case _ => sorry
+case _ => sorry
+case _ => sorry
+case _ => sorry
+case _ => sorry
+case _ => sorry
+case _ => sorry
+case _ => sorry
+case _ => sorry
+case _ => sorry
+case _ => sorry
+case _ => sorry
+case _ => sorry
+case _ => sorry
+case _ => sorry
+case _ => sorry
+case _ => sorry
+case _ => sorry
+case _ => sorry
+case _ => sorry
+case _ => sorry
+case _ => sorry
+case _ => sorry
+case _ => sorry
+case _ => sorry
+case _ => sorry
+case _ => sorry
+case _ => sorry
+case _ => sorry
+case _ => sorry
+case _ => sorry
+case _ => sorry
+case _ => sorry
+case _ => sorry
+case _ => sorry
+case _ => sorry
+case _ => sorry
+case _ => sorry
+case _ => sorry
+case _ => sorry
+case _ => sorry
+case _ => sorry
+case _ => sorry
+case _ => sorry
+case _ => sorry
+case _ => sorry
+case _ => sorry
+case _ => sorry
+case _ => sorry
+case _ => sorry
+case _ => sorry
+case _ => sorry
+case _ => sorry
+case _ => sorry
+case _ => sorry
+case _ => sorry
+case _ => sorry
+case _ => sorry
+case _ => sorry
+case _ => sorry
+case _ => sorry
+case _ => sorry
+case _ => sorry
+case _ => sorry
+case _ => sorry
+case _ => sorry
+case _ => sorry
+
+
+-- case _ => intros; apply Judgment.wfnil;
+-- all_goals try (intro j c; cases j; cases c)
 -- case _ ih wf c =>
 --   apply Judgment.wfempty (ih wf c)
--- case _ ih _ wf _ _ c1 c =>
---   apply Judgment.wfkind;
---   sorry;
---   apply (ih wf c);
--- case _ Γ' _ _ _ _ _ c ih1 ih2 wf h1 _ h2 c1 c2 =>
---   simp at Γ';
+-- case _ Γ' _ c1 ih wf _ j1 c2 =>
 --   apply Judgment.wftype;
---   replace ih1 := ih1 wf c2;
+--   apply (ih Γ' c1);
+--   sorry
+--   sorry
+-- case _ Γ' j1 c1 ih1 wf _ j2 c2 =>
+--   apply Judgment.wfkind;
+--   replace ih1 := ih1 Γ' c1;
 --   apply ih2 Γ' c; assumption;
 --   apply ih1; assumption; assumption;
 -- case _ Γ' _ _ _ _ _ _ h1' ih1 ih2 wf h1 h2 _ c1 c2 =>
@@ -31,6 +173,22 @@ theorem compile_wf_ctx :
 --   have ih2' := ih2 Γ' sorry h1' c2; assumption;
 --   sorry
 --   apply ih1 wf c2
+-- case _ => sorry
+-- case _ => sorry
+-- case _ => sorry
+-- case _ => sorry
+-- case _ => sorry
+-- case _ => sorry
+-- case _ => sorry
+-- case _ => sorry
+-- case _ => sorry
+-- case _ => sorry
+-- case _ => sorry
+-- case _ => sorry
+-- case _ => sorry
+-- case _ => sorry
+-- case _ => sorry
+-- case _ => sorry
 -- case _ => sorry
 -- case _ => sorry
 -- case _ => sorry
@@ -47,22 +205,22 @@ induction x;
 case _ => sorry
 case _ => sorry
 
-@[simp]
-abbrev CompileTypePreservingType : (v : CompileVariant) -> (Γ : Ctx HsTerm) -> CompileJArgs v Γ -> Prop
-| .term => λ Γ => λ ⟨t, τ ; j, t'⟩ => ∀ Γ' τ',
-  ⊢s Γ ->
-  CompileJ .ctx Γ Γ' ->
-  ⊢ Γ' ->
-  (jτ : Γ ⊢s τ : `★) ->
-  CompileJ .term Γ ⟨τ, `★ ; jτ, τ'⟩ ->
-  CompileJ .term Γ ⟨t, τ ; j, t'⟩ ->
-  Γ' ⊢ t' : τ'
-| .ctx => λ _ => λ _ => true
+-- @[simp]
+-- abbrev CompileTypePreservingType : (v : CompileVariant) -> (Γ : Ctx HsTerm) -> CompileJArgs v Γ -> Prop
+-- | .term => λ Γ => λ ⟨t, τ ; j, t'⟩ => ∀ Γ' τ',
+--   ⊢s Γ ->
+--   CompileJ .ctx Γ Γ' ->
+--   ⊢ Γ' ->
+--   (jτ : Γ ⊢s τ : `★) ->
+--   CompileJ .term Γ ⟨τ, `★ ; jτ, τ'⟩ ->
+--   CompileJ .term Γ ⟨t, τ ; j, t'⟩ ->
+--   Γ' ⊢ t' : τ'
+-- | .ctx => λ _ => λ _ => true
 
-theorem compile_type_preserving :
-  CompileJ v Γ idx ->
-  CompileTypePreservingType v Γ idx
- := by sorry
+-- theorem compile_type_preserving :
+--   CompileJ v Γ idx ->
+--   CompileTypePreservingType v Γ idx
+--  := by sorry
 -- intro j; induction j <;> simp at *;
 -- all_goals (intro Γ' τ' wf cc wf' jτ c1 c2)
 -- case _ => sorry
