Hs.lean
@@ -1,5 +1,5 @@
 import Hs.HsTerm
 import Hs.HsJudgment
 import Hs.Algorithm
-import Hs.Compile
+import Hs.CompileJ
 import Hs.Metatheory.Preservation
